src/ADT/ComputationalADT.v
@@ -4,20 +4,33 @@ Require Import Coq.Sets.Ensembles.
 Generalizable All Variables.
 Set Implicit Arguments.
 
-(** Definition of a fully computational ADT *)
+(** Definition of a fully deterministic ADT *)
 
-(** Type of a computational constructor. *)
-Definition cConstructorType (rep dom : Type)
-  :=  dom (* Initialization arguments *)
-     -> rep (* Freshly constructed model *).
+(** Type of a deterministic constructor. *)
+Fixpoint cConstructorType (rep : Type) (dom : list Type)
+  :=
+    match dom with
+    | nil =>
+      rep (* Freshly constructed model *)
+    | cons d dom' =>
+      d -> cConstructorType rep dom' (* Initialization arguments *)
+    end.
 
-(** Type of a method. *)
-Definition cMethodType (rep dom cod : Type)
-  := rep    (* Initial model *)
-     -> dom (* Method arguments *)
-     -> (rep * cod) (* Final model and return value. *).
+(** Type of a deterministic method. *)
+Fixpoint cMethodType' (rep cod : Type)
+           (dom : list Type) : Type :=
+  match dom with
+  | nil =>
+    (prod rep cod) (* Final model and return value *)
+  | cons d dom' =>
+    d -> cMethodType' rep cod dom' (* Method arguments *)
+  end.
+Definition cMethodType (rep : Type)
+           (dom : list Type)
+           (cod : Type) : Type :=
+  rep -> cMethodType' rep cod dom.
 
-(** Interface of a computational ADT *)
+(** Interface of a ADT implementation *)
 Record pcADT (Sig : ADTSig)
        (* Representation Type of the ADT is a parameter to get around
         Universe problems. *)
@@ -36,6 +49,7 @@ Record pcADT (Sig : ADTSig)
                                 (snd (MethodDomCod Sig idx))
   }.
 
+(* Definition of of an ADT implementation *)
 Definition cADT (Sig : ADTSig) := sigT (pcADT Sig).
 Definition cRep {Sig : ADTSig} (c : cADT Sig) : Type := projT1 c.
 Definition cConstructors {Sig : ADTSig} (c : cADT Sig)
@@ -48,7 +62,40 @@ Definition cMethods {Sig : ADTSig} (c : cADT Sig)
               (snd (MethodDomCod Sig idx))
   := pcMethods (projT2 c) idx.
 
+(* Lifting a deterministic ADT to computation-land. *)
+Fixpoint LiftcConstructor
+         (rep : Type) (dom : list Type)
+  : cConstructorType rep dom
+    -> constructorType rep dom :=
+  match dom return
+        cConstructorType rep dom
+        -> constructorType rep dom
+  with
+  | nil => fun cConstructor => ret cConstructor
+  | cons d dom' => fun cConstructor t =>
+                   LiftcConstructor rep dom' (cConstructor t)
+  end.
+
+Fixpoint LiftcMethod'
+         (rep cod : Type) (dom : list Type)
+  : cMethodType' rep cod dom
+    -> methodType' rep cod dom :=
+  match dom return
+        cMethodType' rep cod dom
+        -> methodType' rep cod dom
+  with
+  | nil => fun cMethod => ret cMethod
+  | cons d dom' => fun cMethod t =>
+                     LiftcMethod' rep cod dom' (cMethod t)
+  end.
+
+Definition LiftcMethod
+           (rep : Type) (dom : list Type) (cod : Type)
+           (cMethod : cMethodType rep dom cod)
+  : methodType rep dom cod
+  := fun r => LiftcMethod' rep cod dom (cMethod r).
+
 Definition LiftcADT (Sig : ADTSig) (A : cADT Sig) : ADT Sig :=
   {| Rep                := cRep A;
-     Constructors idx d := ret (cConstructors A idx d);
-     Methods idx r d    := ret (cMethods A idx r d) |}.
+     Constructors idx :=  LiftcConstructor _ _ (cConstructors A idx);
+     Methods idx    := LiftcMethod (cMethods A idx) |}.
