src/ADTNotation/BuildADT.v
@@ -31,18 +31,11 @@ Class CoDHint := {codHint : Type}.
 Record methDef {Rep : Type} (Sig : methSig) :=
   { methBody :> methodType Rep (methDom Sig) (methCod Sig)}.
 
-Notation "'Def' 'Method' id ( r : 'rep' , x : dom ) : cod := bod" :=
-  (Build_methDef {| methID := id; methDom := dom; methCod := cod |} (fun (r : repHint) x => let cod := {| codHint := cod |} in bod%comp))
-    (no associativity, id at level 0, r at level 0, x at level 0, dom at level 0,
-     cod at level 0, only parsing,
-     at level 94, format "'Def'  'Method'  id  ( r  :  'rep' ,  x  :  dom )  :  cod  := '/' '[  '   bod ']' " ) :
-methDefParsing_scope.
-
-Notation "'Def' 'Method' id ( r : 'rep' , x : dom ) : cod := bod" :=
-  (Build_methDef {| methID := id; methDom := dom; methCod := cod |} (fun r x => bod%comp))
-    (no associativity, id at level 0, r at level 0, x at level 0, dom at level 0,
-     cod at level 0,
-     at level 94, format "'Def'  'Method'  id  ( r  :  'rep' ,  x  :  dom )  :  cod  :=  '/' '[  '   bod ']' " ) :
+Notation "'Def' 'Method' id ( r : 'rep' ) x1 .. xn : cod := bod" :=
+  (Build_methDef {| methID := id; methDom := _; methCod := cod |} (fun r => (fun x1 => .. (fun xn =>  bod%comp) ..)))
+    (no associativity, id at level 0, r at level 0, x1 closed binder,
+     xn closed binder, cod at level 0,
+     at level 94, format "'Def'  'Method'  id  (  r  :  'rep'  )  x1  ..  xn  :  cod  :=  '/' '[  '   bod ']' " ) :
 methDef_scope.
 
 Delimit Scope methDefParsing_scope with methDefParsing.
@@ -50,13 +43,6 @@ Delimit Scope methDef_scope with methDef.
 
 Record consDef {Rep : Type} (Sig : consSig) :=
   { consBody :> constructorType Rep (consDom Sig) }.
-
-Notation "'Def' 'Constructor' id ( x : dom ) : 'rep' := bod" :=
-  (Build_consDef {| consID := id; consDom := dom |} (fun x => bod%comp))
-    (no associativity, at level 94, id at level 0,
-     x at level 0, dom at level 0,
-     format "'Def'  'Constructor'  id  ( x :  dom )  :  'rep'  :=  '/' '[  '   bod ']' " ) :
-consDef_scope.
 
 Delimit Scope consDef_scope with consDef.
 
@@ -87,8 +73,8 @@ Definition getMethDef
   methBody (ith methDefs idx).
 
 (* Always simplify method lookup when the index is specified. *)
-Arguments getConsDef [_] {n} [_] _ idx%string / _ _ .
-Arguments getMethDef [_] {n} [_] _ idx%string / _ _ _ .
+Arguments getConsDef [_] {n} [_] _ idx%string / .
+Arguments getMethDef [_] {n} [_] _ idx%string / _ .
 
 (* [BuildADT] constructs an ADT from a single constructor
    definition and a list of method signatures,
@@ -151,3 +137,124 @@ Notation callMeth adt idx := (callADTMethod adt (fun idx => ibound (indexb idx))
                                              {| bindex := idx |}).
 Notation callCons adt idx := (callADTConstructor adt (fun idx => ibound (indexb idx))
                                                   {| bindex := idx |}).
+
+Section CacheADT.
+
+  Variable Key : Type.
+  Variable Value : Type.
+
+  Definition CacheSig : ADTSig :=
+    ADTsignature {
+        Constructor "EmptyCache"  : [ unit : Type ] -> rep,
+        Method "AddKey" : rep x [Key] -> rep x bool ,
+        Method "UpdateKey" : rep x [Key; (Value -> Value)] -> rep x bool ,
+        Method "LookupKey" :  rep x [Key ] -> rep x (option Value)
+  }%ADTSig.
+
+  Definition EnsembleInsert  {A} (a : A) (ens : Ensemble A) (a' : A)
+    : Prop := a' = a \/ ens a'.
+
+  Definition SubEnsembleInsert {A} (a : A) (ens ens' : Ensemble A)
+  : Prop :=
+    forall (a' : A), ens' a' -> EnsembleInsert a ens a'.
+
+  Definition EnsembleRemove
+             (k : Key)
+             (ens : Ensemble (Key * Value))
+             (k' : Key * Value)
+  : Prop := (fst k' <> k /\ ens k').
+
+  Definition EnsembleReplace
+             (k : Key * Value)
+             (ens : Ensemble (Key * Value))
+             (k' : Key * Value)
+  : Prop := k' = k \/
+            (EnsembleRemove (fst k) ens k').
+
+  Definition EnsembleUpdate
+             (k : Key)
+             (ens : Ensemble (Key * Value))
+             (f : Value -> Value)
+             (kv : Key * Value)
+  : Prop := ((fst kv) = k /\ exists v, (snd kv) = f v /\ Ensembles.In _ ens (k, v)) \/
+            (EnsembleRemove k ens kv).
+
+  Lemma SubEnsembleInsertReplace
+  : forall (kv : Key * Value)
+           (r : Ensemble (Key * Value)),
+   SubEnsembleInsert kv r (EnsembleReplace kv r).
+  Proof.
+    unfold SubEnsembleInsert, EnsembleInsert,
+    EnsembleReplace, EnsembleRemove; intros; intuition.
+  Qed.
+
+  Lemma SubEnsembleInsertRefl
+  : forall (kv : Key * Value)
+           (r : Ensemble (Key * Value)),
+   SubEnsembleInsert kv r r.
+  Proof.
+    unfold SubEnsembleInsert, EnsembleInsert,
+    EnsembleReplace, EnsembleRemove; intros; eauto.
+  Qed.
+
+  Definition ValidLookup
+             (r : Ensemble (Key * Value))
+             (k : Key)
+             (v : option Value)
+  : Prop := forall v', v = Some v' -> r (k, v').
+
+  Definition usedKey
+             (r : Ensemble (Key * Value))
+             (k : Key)
+  : Prop := exists v, r (k, v).
+
+Notation "'Def' 'Method' id ( r : 'rep' ) x1 .. xn : cod := bod" :=
+  (Build_methDef {| methID := id; methDom := [_; _ ] ; methCod := cod |} (fun r =>
+                                                                     (fun x1 => .. (fun xn => let cod := {| codHint := cod |} in bod%comp) ..)))
+    (no associativity, id at level 0, r at level 0, x1 closed binder , xn closed binder, dom at level 0,
+     cod at level 0, only parsing,
+     at level 94,
+     format "'Def'  'Method'  id  (  r  :  'rep'  )  x1  ..  xn  :  cod  :=  '/' '[  '   bod ']' ")
+  : methDefParsing_scope.
+
+Notation "'Def' 'Constructor' id x1 .. xn : 'rep' := bod" :=
+  (Build_consDef _ {| consID := id; consDom := (cons tt ( .. (cons tt nil) ..)) |} (fun x1 => .. (fun xn =>  bod%comp ) ..))
+    (no associativity, at level 94, id at level 0,
+     x1 closed binder, xn closed binder,
+     format "'Def'  'Constructor'  id  x1  ..  xn  :  'rep'  :=  '/' '[  '   bod ']' " ) :
+consDef_scope.
+
+
+  Delimit Scope ADTParsing_scope with ADTParsing.
+Print BuildADTSig.
+Notation "'ADTRep' r { cons1 , meth1 , .. , methn } " :=
+  (let _ := {| repHint := r |} in
+   (let g := (@BuildADT r
+             _ _
+             _ _
+             (icons cons1%consDef (@inil _ (@consDef r)))
+             (icons meth1%methDefParsing .. (icons methn%methDefParsing (@inil _ (@methDef r))) ..)) in g))
+    (no associativity, at level 96, r at level 0,
+     format "'ADTRep'  r   '/' '[hv  ' {  cons1 ,  '//' meth1 , '//' .. , '//' methn  ']' }") : ADTParsing_scope.
+
+Definition foozbar := option Value.
+
+  Definition CacheSpec : ADT _ :=
+    (ADTRep (Ensemble (Key * Value)) {
+        Def Constructor "EmptyCache" (t : unit) : rep :=
+          ret (fun _ => False),
+        Def Method "AddKey" (r : rep) (k : Key) (v : Value) : bool :=
+            { r' | (SubEnsembleInsert (k, v) r (fst r')) /\
+                   ((usedKey r k /\ snd r' = false) \/
+                    (~ usedKey r k /\ snd r' = true))},
+        Def Method "UpdateKey" (r : rep) (k : Key) (v : Value -> Value) : bool :=
+              { r' |
+                (Same_set _ (fst r') (EnsembleUpdate k r v))
+                 /\ ((usedKey r k /\ snd r' = true) \/
+                     (~ usedKey r k -> snd r' = false))},
+        Def Method "LookupKey" (r : rep) (k : Key) (v' : Value) : (foozbar) :=
+                v <- {v | ValidLookup r k v};
+        ret (r, v)
+      }%ADTParsing) : ADT _.
+
+End CacheADT.
