src/ADTRefinement.v
@@ -2,3 +2,6 @@ Require Export Fiat.ADTRefinement.Core
         Fiat.ADTRefinement.SetoidMorphisms
         Fiat.ADTRefinement.GeneralRefinements
         Fiat.ADTRefinement.Refinements.
+
+Arguments refineMethod / .
+Arguments refineConstructor / .
